

Winter Lab Meeting – Fall 20/21

Kronecker Lemma and its Application

Statment: Kronecker Lemma

If sequences $a_n \uparrow \infty$ and $\{\sum_{n=1}^m x_n/a_n\}_{m=1}^\infty$ converges, $\lim_{n \rightarrow \infty} a_n^{-1} \sum_{m=1}^n x_m \rightarrow 0$.

Take $a_0 = b_0 = 0$ and for $m \geq 1$, $b_m := \sum_{k=1}^m x_k/a_k$. Then $x_m = a_m(b_m - b_{m-1})$, so

$$a_n^{-1} \sum_{m=1}^n x_m = a_n^{-1} \left\{ a_n b_n + \sum_{m=2}^n a_m b_m - \sum_{m=2}^n a_m b_{m-1} \right\} = b_n - \sum_{m=1}^n \frac{a_m - a_{m-1}}{a_n} b_{m-1}$$

It suffices to show $\lim_{m \rightarrow \infty} \sum_{m=1}^n \frac{a_m - a_{m-1}}{a_n} b_{m-1} = \lim_{n \rightarrow \infty} b_n =: b_\infty$. Take $B := \sup |b_n|$. For $\epsilon > 0$, as $\lim_{m \rightarrow \infty} b_m = b_\infty$, $\exists M \in \mathbb{N}$ s.t. $|b_m - b_\infty|, \forall m \geq M$. As $a_n \uparrow \infty$, $\exists N > M$ s.t. $a_n > 4Ba_m/\epsilon, \forall n \geq N$ (Equivalently, $a_M/a_n < \epsilon/(4B)$).

Noticing that $\sum_{m=1}^k (a_m - a_{m-1}) = a_k - a_0 = a_k$ holds for all $k \in \mathbb{N}$. Then whenever

$$\begin{aligned} n \geq N, & \left| \sum_{m=1}^n \frac{a_m - a_{m-1}}{a_n} b_{m-1} - b_\infty \right| \stackrel{a_{m+1} \geq a_m}{\leq} \sum_{m=1}^n \frac{a_m - a_{m-1}}{a_n} |b_{m-1} - b_\infty| \\ &= \sum_{m=1}^M \frac{a_m - a_{m-1}}{a_n} |b_{m-1} - b_\infty| + \sum_{m=M+1}^n \frac{a_m - a_{m-1}}{a_n} |b_{m-1} - b_\infty| \\ &= \sum_{m=1}^M \frac{a_m - a_{m-1}}{a_n} (2B) + \sum_{m=1}^M \frac{a_m - a_{m-1}}{a_n} \left(\frac{\epsilon}{2} \right) < \left(\frac{\epsilon}{4B} \right) (2B) + \frac{\epsilon}{2} = \epsilon \\ \Rightarrow \lim_{n \rightarrow \infty} a_n^{-1} \sum_{m=1}^n x_m &= \lim_{n \rightarrow \infty} b_n - \lim_{n \rightarrow \infty} \sum_{m=1}^n \frac{a_m - a_{m-1}}{a_n} b_{m-1} = b_\infty - b_\infty = 0. \end{aligned}$$

Generalization of Kronecker Lemma

Kronecker Lemma for Double Series

Let $\{a_{ij}\}_{i,j \in \mathbb{N}^+}$ be a double sequence of positive number s.t.

- $a_{i+1,j} - a_{ij} \geq 0$ and $a_{i,j+1} - a_{ij} \geq 0$ for all i, j .
- $a_{i+1,j+1} - a_{i+1,j} - a_{i,j+1} + a_{ij}$ is of constant sign.
- $a_{ij} \rightarrow \infty$ as $\min(i, j) \rightarrow \infty$.

If $\sum_{i=1}^{\infty} \sum_{j=1}^{\infty} x_{ij}/a_{ij}$ converges, then $a_{mn}^{-1} \sum_{i=1}^m \sum_{j=1}^n x_{ij} \rightarrow 0$ as $\min(i, j) \rightarrow \infty$.

Remark:

- 1 Potentially useful to handling rectangular partial sums in research problems related to spatial setting.
- 2 In the above statement, the convergence of $\{a_{ij}\}_{i,j \in \mathbb{N}^+}$ is defined as following:
 $\{a_{ij}\}_{i,j \in \mathbb{N}^+}$ converges to a iff $\exists a$ s.t. $\forall \epsilon > 0$, $\exists N \in \mathbb{N}$ s.t. whenever $\min(i, j) \geq N$, $|a_{ij} - a| < \epsilon$.
- 3 Refer to [The Kronecker lemmas for multiple series and some applications](#) for further generalizations

Applications of Kronecker Lemma

- 1 Establish SLLN for Martingales.

Kolmogorov's Variance Criterion

Let X_1, X_2, \dots be independent, then (1) $\mathbb{E}(X_n) = 0$ for all n and (2) $\sum_n \mathbb{E}(X_n^2) < \infty$ together implies $\sum_n X_n$ converges a.s.

- 2 Take $a_n = n^c$ in Kronecker Lemma for some $c > 0$. By Variance Criteria, $\mathbb{E}(X_n) = 0$ for all n and $\sum_n \mathbb{E}(n^{-2c} X_n^2) < \infty$ implies $\sum_n n^{-c} X_n$ converges a.s. By Kronecker Lemma, it further implies that $n^{-c} \sum_{k=1}^n X_k \rightarrow 0$ a.s.
Remark: Tune the non-decreasing sequence a_n to obtain desired constraint.